Download Link: https://assignmentchef.com/product/solved-dynamical-homework-7
<br>
<strong>1.1      Section 3.7 Problem 2.</strong>

Observe that the only <em>T</em>-invariant subset of <em>X </em>is <em>X </em>itself. Suppose we have a subset <em>A </em>of <em>X </em>such that <em>A 6</em>= <em>X</em>. Then there exists <em>a<sub>j </sub>∈ X </em>such that <em>a</em><sub>(<em>j</em>+1) mod <em>n </em></sub><em>∈6 A </em>and hence, <em>T</em>(<em>a<sub>j</sub></em>) <em>6∈ A</em>. Thus <em>A </em>is not <em>T</em>-invariant. Hence, we must have <em>A </em>= <em>X</em>. But <em>A<sup>C </sup></em>= <em>X<sup>C </sup></em>= <em>∅</em>. So <em>µ</em>(<em>A<sup>C</sup></em>) = 0 whenever <em>A </em>is <em>T</em>-invariant, and so <em>T </em>is ergodic.

<strong>Problem 3.</strong>

Suppose <em>T </em>is a totally ergodic measure-preserving transformation and suppose that <em>T </em>is invertible. Since <em>T </em>is ergodic, observe that <em>µ</em>(<em>A</em>) = 0 or <em>µ</em>(<em>A<sup>C</sup></em>) = 0 for any <em>T</em>-invariant set <em>A</em>. Now fix a <em>T</em>-invariant set <em>A </em>and suppose <em>µ</em>(<em>A</em>) = 0. Since <em>T </em>is measure-preserving, we have that if <em>µ</em>(<em>A</em>) = 0, then <em>µ</em>(<em>T<sup>−</sup></em><sup>1</sup>(<em>A</em>)) = 0.

For <em>T<sup>−</sup></em><sup>2</sup>(<em>A</em>), observe that we have

<em>T<sup>−</sup></em><sup>2</sup>(<em>A</em>) = <em>T<sup>−</sup></em><sup>1</sup>(<em>T<sup>−</sup></em><sup>1</sup>(<em>A</em>)) = <em>T<sup>−</sup></em><sup>1</sup>(<em>B</em>)

where <em>B </em>= <em>T<sup>−</sup></em><sup>1</sup>(<em>A</em>), a measure 0 set. Again, since <em>T </em>is measure-preserving and <em>µ</em>(<em>B</em>) = 0, we have that <em>µ</em>(<em>T<sup>−</sup></em><sup>1</sup>(<em>B</em>)) = <em>µ</em>(<em>T<sup>−</sup></em><sup>2</sup>(<em>A</em>)) = 0. Proceeding inductively, we get that if <em>µ</em>(<em>A</em>) = 0, then <em>µ</em>(<em>T<sup>n</sup></em>(<em>A</em>)) = 0 for all <em>n &lt; </em>0. Moreover, if <em>A </em>is <em>T</em>-invariant, then <em>A </em>is also <em>T<sup>−</sup></em><sup>1</sup>-invariant, since <em>T </em>is invertible. This again applies for <em>T<sup>n </sup></em>with any <em>n &lt; </em>0, so we have that <strong>Problem 6.</strong>

Recall the the two dimensional Baker’s transformation is defined as

 <em><u><sub>y</sub></u></em>

<sup></sup>(2<em>x, </em>)<em>,        </em>if 0 <em>≤ x &lt; </em>1<em>/</em>2

<em>T</em>(<em>x,y</em>) =              <sub>2</sub>

<em>,      </em>if 1<em>/</em>2 <em>≤ x ≤ </em>1

For any subset <em>A </em>of [0<em>,</em>1] <em>× </em>[0<em>,</em>1], we have that <em>µ</em>(<em>A</em>) =

1

<strong>1.2      Section 3.10 Problem 1.</strong>

<strong>Problem 3.</strong>

<strong>Problem 4.</strong>

<strong>Problem 6.</strong>

2